to solve time-out of Min_leader_decision problem

paxos-consistency.dfy
@@ -34,11 +34,6 @@ module Consistency {
         && (forall c :: c in leaders ==> s.promise_count[c] <= acceptors)
         && (forall a, c :: a in acceptors && c in leaders && a in s.promise_count[c] ==> (exists h :: PMsg(s.leader_ballot[c], h, 0) in s.pmsgs[a]))
         && (forall a :: a in acceptors ==> s.acceptor_state[a].value >= 0)
-        // the following invariant is to resolve the assertion in base case of lemma Min_leader_decision
-        && s.ballot >= 0 && s.ballot == |s.ballot_mapping|
-        && (forall c :: c in leaders && s.leader_ballot[c] >= 0 ==> s.leader_ballot[c] < |s.ballot_mapping|)
-        && (forall c :: c in leaders && s.leader_ballot[c] >= 0 ==> s.ballot_mapping[s.leader_ballot[c]] == c)
-        && (forall c1, c2 :: c1 in leaders && c2 in leaders && s.leader_ballot[c1] == s.leader_ballot[c2] > 0 ==> c1 == c2)
 //        && (forall a :: a in acceptors ==> !(PMsg(-1, -1, 0) in s.pmsgs[a])) //
 //        && (forall a :: a in acceptors ==> s.acceptor_ballot[a] <= s.acceptor_state[a].highest) //
 //        && (forall a, bn, value :: a in acceptors && CMsg(bn, value) in s.cmsgs[a] ==> bn <= s.acceptor_ballot[a]) //
@@ -68,6 +63,16 @@ module Consistency {
            h < bn && (exists n :: n in leaders && 0 <= s.leader_ballot[n] <= h && s.leader_propose[n] == v)) // * invariant Y
     }
 
+    // the following are invariants used in the proof of lemma Same_ballot_leaders (split from the main body of invariants)
+    ghost predicate valid_leader_ballot(s: TSState) 
+    requires type_ok(s)
+    {
+        && s.ballot >= 0 && s.ballot == |s.ballot_mapping|
+        && (forall c :: c in leaders && s.leader_ballot[c] >= 0 ==> s.leader_ballot[c] < |s.ballot_mapping|)
+        && (forall c :: c in leaders && s.leader_ballot[c] >= 0 ==> s.ballot_mapping[s.leader_ballot[c]] == c)
+        && (forall c1, c2 :: c1 in leaders && c2 in leaders && s.leader_ballot[c1] == s.leader_ballot[c2] > 0 ==> c1 == c2)
+    }
+
     lemma Conflict_confirm_promise(s: TSState, c1: Acceptor, c2: Acceptor)
     requires type_ok(s) && valid(s)
     requires c1 in leaders && c2 in leaders
@@ -86,9 +91,24 @@ module Consistency {
         //assert s.promise_count[c2] <= (set a | a in acceptors && (exists h :: PMsg(s.leader_ballot[c2], h, 0) in s.pmsgs[a]));
         SubsetSize(s.promise_count[c2], (set a | a in acceptors && (exists h :: PMsg(s.leader_ballot[c2], h, 0) in s.pmsgs[a])));
     }
+    // the base case of lemma Min_leader_decision
+    lemma Same_ballot_leaders(s: TSState, c1: Acceptor, c2: Acceptor)
+    requires type_ok(s) && valid(s) && valid_leader_ballot(s)
+    requires c1 in leaders && c2 in leaders
+    requires s.leader_ballot[c1] == s.leader_ballot[c2] >= 0
+    ensures c1 == c2
+    {}
+    // selecting a leader with the same proposal but a smaller ballot number in the induction step of lemma Min_leader_decision
+    lemma Select_leader_smaller_ballot(s: TSState, c1: Acceptor) returns (c2: Acceptor)
+    requires type_ok(s) && valid(s) && c1 in leaders
+    requires s.leader_propose[c1] > 0 && |s.promise_count[c1]| <= F
+    ensures c2 in leaders && s.leader_ballot[c2] < s.leader_ballot[c1] && s.leader_propose[c2] == s.leader_propose[c1]
+    {
+        c2 :| c2 in leaders && s.leader_ballot[c2] < s.leader_ballot[c1] && s.leader_propose[c2] == s.leader_propose[c1];
+    }
 
     // lemma Min_leader_decision(s: TSState, c1: Acceptor, c2: Acceptor)
-    // requires type_ok(s) && valid(s)
+    // requires type_ok(s) && valid(s) && valid_leader_ballot(s)
     // requires c1 in leaders && c2 in leaders
     // requires s.leader_ballot[c1] <= s.leader_ballot[c2]
     // requires s.leader_propose[c1] > 0 && s.leader_propose[c2] > 0
@@ -96,17 +116,19 @@ module Consistency {
     // requires forall c :: c in leaders  && s.leader_ballot[c] < s.leader_ballot[c1] ==> 
     //     (|set a | a in acceptors && CMsg(s.leader_ballot[c], s.leader_propose[c]) in s.cmsgs[a]| <= F)
     // ensures s.leader_propose[c1] == s.leader_propose[c2]
+    // //invariant s.leader_ballot[1] <= s.leader_ballot[2]
     // decreases s.leader_ballot[c2] - s.leader_ballot[c1]
     // {
     //     if s.leader_ballot[c2] == s.leader_ballot[c1]{
     //         // base case: when c2 == c1, then their proposal should be the same
-    //         assert c1 == c2;
+    //         // assert c1 == c2;
     //     } else { 
     //         // induction step:
-    //         assert s.leader_ballot[c2] > s.leader_ballot[c1];
+    //         //assert s.leader_ballot[c2] > s.leader_ballot[c1];
     //         Conflict_confirm_promise(s, c1, c2); // rule out the first case of invariant X
-    //         assert exists c :: c in leaders && s.leader_ballot[c] < s.leader_ballot[c2] && s.leader_propose[c] == s.leader_propose[c2];
-    //         var c3 :| c3 in leaders && s.leader_ballot[c3] < s.leader_ballot[c2] && s.leader_propose[c3] == s.leader_propose[c2]; // this is from the second case of invariant X and invariant Y
+    //         //assert exists c :: c in leaders && s.leader_ballot[c] < s.leader_ballot[c2] && s.leader_propose[c] == s.leader_propose[c2];
+    //         //var c3 :| c3 in leaders && s.leader_ballot[c3] < s.leader_ballot[c2] && s.leader_propose[c3] == s.leader_propose[c2]; // this is from the second case of invariant X and invariant Y
+    //         var c3 := Select_leader_smaller_ballot(s, c2);
     //         Min_leader_decision(s, c1, c3);
     //     }
     // }
